

MATH22981 - Regression Supplement

Anthony Tan

December 10th, 2016

The objective is to convert a non-linear problem to a linear problem. Some basic non-linear equations you may already know include

$$y = ax^k, \quad (1)$$

$$y = a(b^{kx}), b > 0 \quad (2)$$

The transformation we are applying is the natural logarithm. That is, if we take the natural logarithm of both sides of equation (1), we have

$$\begin{aligned} \ln y &= \ln(ax^n) \\ \ln y &= \ln a + \ln x^k \\ \ln y &= \ln a + k \ln x \\ Y &= \ln a + kX \end{aligned} \quad (3)$$

where $X = \ln x$ and $Y = \ln y$. Similarly for equation (2), we have

$$\begin{aligned} \ln y &= \ln(a(b)^{kx}) \\ \ln y &= \ln a + \ln b^{kx} \\ \ln y &= \ln a + kx \ln b \\ Y &= \ln a + (k \ln b)X \end{aligned} \quad (4)$$

where $X = x$ and $Y = \ln y$. **Keep in mind, if you are using \log to some base, b , the same rules apply. However, if you are trying to solve for certain variables, you have to keep in mind the base you are working with. I chose to use the natural logarithm because the calculations are simpler.**

Using the method of least squares for equation (3), we can find our k and a value by the following formulas

$$k = \frac{n \sum XY - \sum X \sum Y}{n \sum X^2 - (\sum X)^2} \quad (5)$$

$$\ln a = \frac{\sum X^2 \sum Y - \sum X \sum XY}{n \sum X^2 - (\sum X)^2} \quad (6)$$

$$(7)$$

Keep in mind, to find a , you must raise both sides apply e to both sides.

Using the method of least squares for equation (4), we can find our k and a value by the following for-

mulas

$$k \ln b = \frac{n \sum XY - \sum X \sum Y}{n \sum X^2 - (\sum X)^2}$$
$$k = \frac{1}{\ln b} \frac{n \sum XY - \sum X \sum Y}{n \sum X^2 - (\sum X)^2} \quad (8)$$

$$\ln a = \frac{\sum X^2 \sum Y - \sum X \sum XY}{n \sum X^2 - (\sum X)^2} \quad (9)$$

Keep in mind, to find a , you must raise both sides apply e to both sides.